working on decoding, need some helper lemmas

Varint.fst
@@ -26,19 +26,57 @@ let rec valid (v:list UInt8.t) : bool =
        which is equivalent to the number fitting into 7 bits *)
   | msb :: [] -> UInt.fits (U8.v msb) 7
     (* Otherwise the continuation bit should be one *)
-    (* Note that U.msb is "most significant bit" while the msb is the patter match is "most significant byte" *)
+    (* Note that U.msb is "most significant bit" while the msb in the pattern match is "most significant byte" *)
   | msb :: rest -> U.msb (U8.v msb) && valid rest
 
 let varint = v:list UInt8.t{length v >= 1 /\ valid v}
 
+let zero_extend_m_vec (#n:pos) (a:BitVector.bv_t n) (m:pos): Tot (BitVector.bv_t (n+m)) = 
+  Seq.append (create m false) a
 
+let zero_extend_m (#n:pos) (a:uint_t n) (m:pos): Tot (uint_t (n+m)) = 
+  from_vec (zero_extend_m_vec (to_vec a) m)
+
+val logand_append: #n:pos -> #m:pos -> a:BitVector.bv_t n -> b:BitVector.bv_t n -> 
+                    c:BitVector.bv_t m -> d:BitVector.bv_t m ->
+                    Lemma (ensures Seq.append (BitVector.logand_vec a b) (BitVector.logand_vec c d) =
+                                   BitVector.logand_vec #(n+m) (Seq.append a c) (Seq.append b d))
+
+val logand_trunc_lemma: #n:pos -> a:uint_t n -> m:pos ->
+  Lemma (requires U.size a m /\ m <= n) (ensures (U.logand a (U.to_uint_t n (U.max_int m))) = a)
+
+let logand_trunc_lemma #n a m = 
+  let b = U.max_int m in
+  let b' = U.to_uint_t m b in
+  let b'' = U.to_uint_t n b in
+  let a' = U.to_uint_t m a in
+  FStar.Math.Lemmas.pow2_le_compat n m;
+  FStar.Math.Lemmas.modulo_lemma b (pow2 n);
+  FStar.Math.Lemmas.modulo_lemma b (pow2 m);
+  assert b' = b'';
+  FStar.Math.Lemmas.modulo_lemma a (pow2 m);
+  assert a = a';
+  UInt.logand_lemma_2 a';
+  assert U.logand a b'' = a;
+  assert True
+  
+  
 let rec encode (x: U64.t) : Tot varint (decreases (U64.v x)) = 
   let nextByte = Cast.uint64_to_uint8 (U64.logand x 0x7FuL) in 
   let rest = U64.(x >>^ 7ul) in
   UInt.logand_le (U64.v x) 0x7F;
-  assert UInt.fits U8.(v nextByte) 7;
   if U64.(lte rest 0uL) then 
-    [nextByte]
+    (
+        assert UInt.fits U8.(v nextByte) 7;
+        UInt.shift_right_value_lemma (U64.v x) 7;
+        assert op_Division (U64.v x) 128 = 0;
+        assert (U64.v x) < 128;
+        assert (U8.v nextByte) < 128;
+        assert (UInt.to_uint_t 7 (U64.v x)) = U64.v x;
+        // UInt.logand_lemma_2 (UInt.to_uint_t)
+        assert U8.v nextByte = U64.v x;
+        [nextByte]
+    )
   else 
     let nextByte = U8.(nextByte +^ 128uy) in
     UInt.shift_right_value_lemma (U64.v x) 7;
@@ -48,11 +86,17 @@ let rec encode (x: U64.t) : Tot varint (decreases (U64.v x)) =
     UInt.lemma_msb_pow2 (U8.v nextByte);
     List.append [nextByte] restEnc
 
-let rec decode (bs:varint) (x:erased U64.t{bs == encode(x)}) : y:U64.t{y == reveal x} =
+
+let rec decode (bs:varint) (x:erased U64.t{bs = encode(reveal x)}) : y:U64.t{y = reveal x} =
   let nextByte = hd bs in
   match U.msb (U8.v nextByte) with 
-  | true -> Cast.uint8_to_uint64 nextByte
-  | false -> 0uL
+  | false -> assert length bs = 1; 
+            // UInt.logand_le (U64.v x) 0x7F;
+            // assert nextByte = Cast.uint64_to_uint8 (U64.logand (reveal x) 0x7FuL);
+            // UInt.logand_mask (U64.v x) 8;
+            // assert U64.v (reveal x) < 128;
+            assert U8.v nextByte = U64.v (reveal x);
+            Cast.uint8_to_uint64 nextByte
+  | true -> 0uL
   
-
 (* Relevant F* code in ASN1*: ANS1.Spec.IdentifierU32.fst *)
